Coq/Simplicity/SHA256.v
@@ -455,8 +455,8 @@ Hint Immediate hashBlock_Parametric : parametricity.
 
 Require Import Simplicity.MerkleRoot.
 
-Fact Hash256_hashBlock : map Byte.unsigned (hash256_to_bytelist (commitmentRoot hashBlock)) =
-  map Byte.unsigned (sha.functional_prog.hexstring_to_bytelist "d753d5f32c88d3503fc450088cc7c82ef5eb2ae669e5ad3149f3f18a9b85ec5b").
+Fact identityRoot_hashBlock : map Byte.unsigned (hash256_to_bytelist (identityRoot hashBlock)) =
+  map Byte.unsigned (sha.functional_prog.hexstring_to_bytelist "da10f0e8530695d07564f0b32feebe77265a1d69cf802e22d77289daf6641b8d").
 Proof.
 vm_compute.
 reflexivity.
